block_equiv_checker.v
@@ -165,6 +165,11 @@ Require Import FORVES.optimizations.and_and_mask.
 Import Opt_and_and_mask.
 Require Import FORVES.optimizations.and_shr.
 Import Opt_and_shr.
+Require Import FORVES.optimizations.add_reshape.
+Import Opt_add_reshape.
+Require Import FORVES.optimizations.shr_and.
+Import Opt_shr_and.
+
 
 Require Import FORVES.symbolic_execution.
 Import SymbolicExecution.
@@ -238,9 +243,6 @@ Import MemoryOpsSolversImplSoundness.
 
 Require Import FORVES.symbolic_state_cmp_soundness.
 Import SymbolicStateCmpSoundness.
-
-Require Import FORVES.optimizations_ext_def.
-Import Optimizations_Ext_Def.
 
 Require Import FORVES.misc.
 Import Misc.
@@ -379,8 +381,8 @@ Module BlockEquivChecker.
   
   
 Inductive available_optimization_step :=
-| OPT_eval
 | OPT_add_zero
+| OPT_eval
 | OPT_not_not
 | OPT_and_and
 | OPT_and_origin
@@ -456,6 +458,10 @@ Inductive available_optimization_step :=
 | OPT_shl_shr
 | OPT_and_and_mask
 | OPT_and_shr
+
+(* Extended optimization rules *)
+| OPT_add_reshape
+| OPT_shr_and
 .
 
 
@@ -463,8 +469,8 @@ Definition list_opt_steps := list available_optimization_step.
 
 Definition get_optimization_step (tag: available_optimization_step) : opt_entry :=
 match tag with 
-| OPT_eval => OpEntry optimize_eval_sbinding optimize_eval_sbinding_snd
 | OPT_add_zero => OpEntry optimize_add_zero_sbinding optimize_add_zero_sbinding_snd
+| OPT_eval => OpEntry optimize_eval_sbinding optimize_eval_sbinding_snd
 | OPT_not_not => OpEntry optimize_not_not_sbinding optimize_not_not_sbinding_snd
 | OPT_and_and => OpEntry optimize_and_and_sbinding optimize_and_and_sbinding_snd
 | OPT_and_origin => OpEntry optimize_and_origin_sbinding optimize_and_origin_sbinding_snd
@@ -540,9 +546,13 @@ match tag with
 | OPT_shl_shr => OpEntry optimize_shl_shr_sbinding optimize_shl_shr_sbinding_snd
 | OPT_and_and_mask => OpEntry optimize_and_and_mask_sbinding optimize_and_and_mask_sbinding_snd
 | OPT_and_shr => OpEntry optimize_and_shr_sbinding optimize_and_shr_sbinding_snd
+
+| OPT_add_reshape => OpExtEntry optimize_add_reshape_sbinding optimize_add_reshape_sbinding_snd
+| OPT_shr_and => OpExtEntry optimize_shr_and_sbinding optimize_shr_and_sbinding_snd
 end.
 
-Definition all_optimization_steps := 
+(* Optimization steps useful for gas optimizers *)
+Definition gas_pipeline := 
   [
    OPT_eval
    ;OPT_add_zero
@@ -593,7 +603,160 @@ Definition all_optimization_steps :=
    ;OPT_iszero2_gt
    ;OPT_iszero2_lt
    ;OPT_iszero2_eq
-   ;OPT_iszero2_slt
+   ;OPT_xor_x_x
+   ;OPT_xor_zero
+   ;OPT_xor_xor
+   ;OPT_or_or
+   ;OPT_or_and
+   ;OPT_and_or
+   ;OPT_and_not
+   ;OPT_or_not
+   ;OPT_or_x_x
+   ;OPT_and_x_x
+   ;OPT_or_zero
+   ;OPT_or_ffff
+   ;OPT_and_ffff
+   ;OPT_and_coinbase
+   ;OPT_balance_address
+   ;OPT_slt_x_x
+   ;OPT_sgt_x_x
+ 
+   ;OPT_jumpi_eval
+   ;OPT_mem_solver
+   ;OPT_strg_solver
+
+].
+
+
+(* Optimization steps useful for size optimizers *)
+Definition size_pipeline := 
+  [
+    OPT_div_shl
+    ;OPT_mul_shl
+    ;OPT_eval
+    ;OPT_add_zero
+    ;OPT_not_not
+    ;OPT_and_and
+    ;OPT_and_origin 
+    ;OPT_shr_zero_x 
+    ;OPT_shr_x_zero
+    ;OPT_eq_zero 
+    ;OPT_sub_x_x 
+    ;OPT_and_zero 
+    ;OPT_div_one 
+    ;OPT_lt_x_one
+    ;OPT_gt_one_x
+    ;OPT_and_address
+    ;OPT_mul_one
+    ;OPT_iszero_gt
+    ;OPT_eq_iszero
+    ;OPT_and_caller
+    ;OPT_iszero3
+    ;OPT_add_sub
+    ;OPT_shl_zero_x
+    ;OPT_sub_zero
+    ;OPT_shl_x_zero
+    ;OPT_mul_zero
+    ;OPT_div_x_x   (* TODO:  useless: checking X <> 0 requires X to be a value
+                           so DIV(X,X) contains constants and will be avaluated
+                           by the "eval" optimization *)
+   ;OPT_div_zero
+   ;OPT_mod_one
+   ;OPT_mod_zero
+   ;OPT_mod_x_x
+   ;OPT_exp_x_zero
+   ;OPT_exp_x_one
+   ;OPT_exp_one_x
+   ;OPT_exp_zero_x
+   ;OPT_exp_two_x
+   ;OPT_gt_zero_x
+   ;OPT_gt_x_x
+   ;OPT_lt_x_zero
+   ;OPT_lt_x_x
+   ;OPT_eq_x_x
+   ;OPT_iszero_sub
+   ;OPT_iszero_lt
+   ;OPT_iszero_xor
+   ;OPT_iszero2_gt
+   ;OPT_iszero2_lt
+   ;OPT_iszero2_eq
+   ;OPT_xor_x_x
+   ;OPT_xor_zero
+   ;OPT_xor_xor
+   ;OPT_or_or
+   ;OPT_or_and
+   ;OPT_and_or
+   ;OPT_and_not
+   ;OPT_or_not
+   ;OPT_or_x_x
+   ;OPT_and_x_x
+   ;OPT_or_zero
+   ;OPT_or_ffff
+   ;OPT_and_ffff
+   ;OPT_and_coinbase
+   ;OPT_balance_address
+   ;OPT_slt_x_x
+   ;OPT_sgt_x_x
+
+   ;OPT_jumpi_eval
+   ;OPT_mem_solver
+   ;OPT_strg_solver
+].
+
+
+(* Optimization steps useful for solc optimizer *)
+Definition solc_pipeline := 
+  [
+    OPT_div_shl
+    ;OPT_mul_shl
+    ;OPT_eval
+    ;OPT_add_zero
+    ;OPT_not_not
+    ;OPT_and_and
+    ;OPT_and_origin 
+    ;OPT_shr_zero_x 
+    ;OPT_shr_x_zero
+    ;OPT_eq_zero 
+    ;OPT_sub_x_x 
+    ;OPT_and_zero 
+    ;OPT_div_one 
+    ;OPT_lt_x_one
+    ;OPT_gt_one_x
+    ;OPT_and_address
+    ;OPT_mul_one
+    ;OPT_iszero_gt
+    ;OPT_eq_iszero
+    ;OPT_and_caller
+    ;OPT_iszero3
+    ;OPT_add_sub
+    ;OPT_shl_zero_x
+    ;OPT_sub_zero
+    ;OPT_shl_x_zero
+    ;OPT_mul_zero
+    ;OPT_div_x_x   (* TODO:  useless: checking X <> 0 requires X to be a value
+                           so DIV(X,X) contains constants and will be avaluated
+                           by the "eval" optimization *)
+   ;OPT_div_zero
+   ;OPT_mod_one
+   ;OPT_mod_zero
+   ;OPT_mod_x_x
+   ;OPT_exp_x_zero
+   ;OPT_exp_x_one
+   ;OPT_exp_one_x
+   ;OPT_exp_zero_x
+   ;OPT_exp_two_x
+   ;OPT_gt_zero_x
+   ;OPT_gt_x_x
+   ;OPT_lt_x_zero
+   ;OPT_lt_x_x
+   ;OPT_eq_x_x
+   ;OPT_iszero_sub
+   ;OPT_iszero_lt
+   ;OPT_iszero_xor
+   ;OPT_iszero2_gt
+   ;OPT_iszero2_lt
+   ;OPT_iszero2_eq
+   ;OPT_iszero2_slt  (* added *)
    ;OPT_xor_x_x
    ;OPT_xor_zero
    ;OPT_xor_xor
@@ -619,94 +782,13 @@ Definition all_optimization_steps :=
    ;OPT_shl_shr
    ;OPT_and_and_mask
    ;OPT_and_shr
-   
+
    ;OPT_jumpi_eval
    ;OPT_mem_solver
    ;OPT_strg_solver
 
-].
-
-Definition all_optimization_steps' := 
-  [OPT_div_shl;
-   OPT_mul_shl;
-   OPT_eval; 
-   OPT_add_zero; 
-   OPT_not_not; 
-   OPT_and_and;    
-   OPT_and_origin; 
-   OPT_shr_zero_x; 
-   OPT_shr_x_zero; 
-   OPT_eq_zero; 
-   OPT_sub_x_x; 
-   OPT_and_zero; 
-   OPT_div_one; 
-   OPT_lt_x_one; 
-   OPT_gt_one_x; 
-   OPT_and_address; 
-   OPT_mul_one; 
-   OPT_iszero_gt; 
-   OPT_eq_iszero;
-   OPT_and_caller;
-   OPT_iszero3;
-   OPT_add_sub;
-   OPT_shl_zero_x;
-   OPT_sub_zero;
-   OPT_shl_x_zero;
-   OPT_mul_zero;
-   OPT_div_x_x;  (* TODO:  useless: checking X <> 0 requires X to be a value
-                           so DIV(X,X) contains constants and will be avaluated
-                           by the "eval" optimization *)
-   OPT_div_zero;
-   OPT_mod_one;
-   OPT_mod_zero;
-   OPT_mod_x_x;
-   OPT_exp_x_zero;
-   OPT_exp_x_one;
-   OPT_exp_one_x;
-   OPT_exp_zero_x;
-   OPT_exp_two_x;
-   OPT_gt_zero_x;
-   OPT_gt_x_x;
-   OPT_lt_x_zero;
-   OPT_lt_x_x;
-   OPT_eq_x_x;
-   OPT_iszero_sub;
-   OPT_iszero_lt;
-   OPT_iszero_xor;
-   OPT_iszero2_gt;
-   OPT_iszero2_lt;
-   OPT_iszero2_eq;
-   (* OPT_iszero2_slt; *)
-   OPT_xor_x_x;
-   OPT_xor_zero;
-   OPT_xor_xor;
-   OPT_or_or;
-   OPT_or_and;
-   OPT_and_or;
-   OPT_and_not;
-   OPT_or_not;
-   OPT_or_x_x;
-   OPT_and_x_x;
-   OPT_or_zero;
-   OPT_or_ffff;
-   OPT_and_ffff;
-   OPT_and_coinbase;
-   OPT_balance_address;
-   OPT_slt_x_x;
-   OPT_sgt_x_x
-
-   (*;OPT_sub_const
-   ;OPT_add_add_const
-   ;OPT_iszero2_lt_zero
-   ;OPT_gt_x_zero_lt
-   ;OPT_iszero2_slt
-   ;OPT_shl_shr
-   ;OPT_and_and_mask
-   ;OPT_and_shr*)
-
-   ;OPT_jumpi_eval
-   ;OPT_mem_solver
-   ;OPT_strg_solver   
+   ;OPT_add_reshape
+   ;OPT_shr_and
 ].
 
   
@@ -751,8 +833,6 @@ Definition evm_eq_block_chkr'
           let sstack_value_cmp := sstack_value_cmp_1 maxid in
           
           (* Combines standard optimization and extended optimizations *)
-          (*let opt := apply_opt_combined_n_times_pipeline_k opt_pipeline test_opt_ext_pipeline
-                     sstack_value_cmp opt_step_rep opt_pipeline_rep in*)
           let opt := apply_opt_n_times_pipeline_k opt_pipeline 
                        sstack_value_cmp opt_step_rep 
                        opt_pipeline_rep in
