block_equiv_checker_facts.v
@@ -122,8 +122,7 @@ Lemma evm_eq_block_chkr'_snd: forall
     safe_sstack_value_cmp_wrt_others sstack_value_cmp_ext ->
 
     eq_block_chkr_snd (evm_eq_block_chkr' memory_updater storage_updater mload_solver sload_solver sstack_value_cmp_ext smemory_cmp_ext sstorage_cmp_ext sha3_cmp_ext opt_pipeline opt_step_rep opt_pipeline_rep).
-Admitted.    
-(*Proof.
+Proof.
   intros memory_updater storage_updater mload_solver sload_solver sstack_value_cmp_ext smemory_cmp_ext sstorage_cmp_ext sha3_cmp_ext opt_pipeline opt_step_rep opt_pipeline_rep H_smemory_updater_ext_snd H_sstorage_updater_ext_snd H_mload_solver_ext_snd H_sload_solver_ext_snd H_sstack_val_cmp_fail_for_d_eq_0 H_safe_smemory_cmp_ext_wrt_sstack_value_cmp H_safe_sstorage_cmp_ext_wrt_sstack_value_cmp H_safe_sha3_cmp_ext_wrt_sstack_value_cmp H_safe_sstack_value_cmp_wrt_others.
 
   (* combining the comparators results in a sound one *)
@@ -308,7 +307,6 @@ Admitted.
     rewrite H_sstate_cmp_snd_2.
     apply eq_execution_states_refl.
 Qed.
-*)
 
 Lemma evm_eq_block_chkr_lazy_snd:
   forall (memory_updater_tag: available_smemory_updaters) (storage_updater_tag: available_sstorage_updaters) (mload_solver_tag: available_mload_solvers) 
