optimizations/shr_and.v
@@ -1,0 +1,110 @@
+Require Import bbv.Word.
+Require Import Nat. 
+Require Import Coq.NArith.NArith.
+Require Import Coq.Bool.Bool.
+
+Require Import Coq.Logic.FunctionalExtensionality.
+
+Require Import FORVES.constants.
+Import Constants.
+
+Require Import FORVES.symbolic_state.
+Import SymbolicState.
+
+Require Import FORVES.symbolic_state_eval.
+Import SymbolicStateEval.
+
+Require Import FORVES.symbolic_state_cmp.
+Import SymbolicStateCmp.
+
+Require Import FORVES.valid_symbolic_state.
+Import ValidSymbolicState.
+
+Require Import FORVES.execution_state.
+Import ExecutionState.
+
+Require Import FORVES.stack_operation_instructions.
+Import StackOpInstrs.
+
+Require Import FORVES.program.
+Import Program.
+
+Require Import FORVES.symbolic_state_cmp_impl.
+Import SymbolicStateCmpImpl.
+
+Require Import FORVES.symbolic_state_eval_facts.
+Import SymbolicStateEvalFacts.
+
+Require Import FORVES.valid_symbolic_state.
+Import ValidSymbolicState.
+
+Require Import FORVES.misc.
+Import Misc.
+
+Require Import FORVES.eval_common.
+Import EvalCommon.
+
+Require Import FORVES.concrete_interpreter.
+Import ConcreteInterpreter.
+
+Require Import FORVES.optimizations_def.
+Import Optimizations_Def.
+
+Require Import FORVES.optimizations_common.
+Import Optimizations_Common.
+
+Require Import List.
+Import ListNotations.
+
+
+Module Opt_shr_and.
+
+
+(* EXTENDED OPTIMIZATION RULE *)
+
+(* SHR(B, AND(X, A)) = AND(SHR(B, X), A >> B) with A, B constants 
+https://github.com/ethereum/solidity/blob/abc46f309676637164076ca1a5b805cd90635bfa/libevmasm/RuleList.h#L558
+*)
+Definition optimize_shr_and_sbinding : opt_ext_smap_value_type := 
+fun (val: smap_value) =>
+fun (fcmp: sstack_val_cmp_t) =>
+fun (sb: sbindings) =>
+fun (maxid: nat) =>
+fun (instk_height: nat) =>
+fun (ops: stack_op_instr_map) => 
+match val with
+| SymOp SHR [b; arg] => 
+  match follow_to_val b maxid sb with
+  | Some bval => 
+    match follow_in_smap arg maxid sb with
+    | Some (FollowSmapVal (SymOp AND [arg1; arg2]) idx' sb') =>
+      match follow_to_val arg1 idx' sb' with
+      | Some aval => 
+        let c := NToWord EVMWordSize (N.shiftr (wordToN aval) (wordToN bval)) in
+        (SymOp AND [Val c; FreshVar maxid], 
+         [(maxid, SymOp SHR [Val bval; arg2])],
+         true)
+      | _ => 
+        match follow_to_val arg2 idx' sb' with
+        | Some aval => 
+          let c := NToWord EVMWordSize (N.shiftr (wordToN aval) (wordToN bval)) in
+          (SymOp AND [Val c; FreshVar maxid], 
+           [(maxid, SymOp SHR [Val bval; arg1])],
+           true)
+        | None => (val, [], false)
+        end 
+      end
+    | _ => (val, [], false)
+    end
+  | _ => (val, [], false)
+  end
+| _ => (val, [], false)
+end.
+
+
+Lemma optimize_shr_and_sbinding_snd : opt_ext_sbinding_snd optimize_shr_and_sbinding.
+Proof.
+Admitted.
+
+
+End Opt_shr_and.
